examples/wysteria/sem.fst
@@ -14,6 +14,9 @@ open FStar.OrdSet
 open Prins
 open AST
 
+(* pre returns comp, for src it's never Skip *)
+type comp = | Do | Skip | NA
+
 (* TODO: FIXME: workaround for projectors *)
 val e_of_t_exp: t:term{is_T_exp t} -> Tot exp
 let e_of_t_exp (T_exp e) = e
@@ -22,147 +25,8 @@ let e_of_t_exp (T_exp e) = e
 val e_of_exp: exp -> Tot exp'
 let e_of_exp (Exp e _) = e
 
-let pre_easpar (c:config) =
-  is_T_exp (t_of_conf c) && is_E_aspar (e_of_exp (e_of_t_exp (t_of_conf c))) && is_par c
-  
-let pre_ebox (c:config) =
-  is_T_exp (t_of_conf c) && is_E_box (e_of_exp (e_of_t_exp (t_of_conf c)))
-
-let pre_eapp (c:config) =
-  is_T_exp (t_of_conf c) && is_E_app (e_of_exp (e_of_t_exp (t_of_conf c)))
-
-let pre_eabs (c:config) =
-  is_T_exp (t_of_conf c) && is_E_abs (e_of_exp (e_of_t_exp (t_of_conf c)))
- 
-let pre_efix (c:config) =
-  is_T_exp (t_of_conf c) && is_E_fix (e_of_exp (e_of_t_exp (t_of_conf c)))
-
-let pre_eempabs (c:config) =
-  is_T_exp (t_of_conf c) && is_E_empabs (e_of_exp (e_of_t_exp (t_of_conf c)))
-
-let pre_elet (c:config) =
-  is_T_exp (t_of_conf c) && is_E_let (e_of_exp (e_of_t_exp (t_of_conf c)))
-
-(* TODO: FIXME: workaround for projectors *)
-val x_of_e_var: e:exp'{is_E_var e} -> Tot varname
-let x_of_e_var (E_var x) = x
-
-(* TODO: FIXME: workaround for projectors *)
-val is_Some: option 'a -> Tot bool
-let is_Some x = match x with
-  | Some _ -> true
-  | _      -> false
-
-(* TODO: FIXME: workaround for projectors *)
-val en_of_conf: config -> Tot env
-let en_of_conf (Conf _ _ _ en _ _) = en
-
-let pre_evar (c:config) =
-  is_T_exp (t_of_conf c) && is_E_var (e_of_exp (e_of_t_exp (t_of_conf c))) &&
-  is_Some ((en_of_conf c) (x_of_e_var (e_of_exp (e_of_t_exp (t_of_conf c)))))
-
-let pre_econst (c:config) =
-  is_T_exp (t_of_conf c) && is_E_const (e_of_exp (e_of_t_exp (t_of_conf c)))
-
-let pre_eunbox (c:config) =
-  is_T_exp (t_of_conf c) && is_E_unbox (e_of_exp (e_of_t_exp (t_of_conf c)))
- 
-let pre_emkwire (c:config) =
-  is_T_exp (t_of_conf c) && is_E_mkwire (e_of_exp (e_of_t_exp (t_of_conf c)))
-
-let pre_eprojwire (c:config) =
-  is_T_exp (t_of_conf c) && is_E_projwire (e_of_exp (e_of_t_exp (t_of_conf c)))
- 
-let pre_econcatwire (c:config) =
-  is_T_exp (t_of_conf c) && is_E_concatwire (e_of_exp (e_of_t_exp (t_of_conf c)))
- 
-let pre_effi (c:config) =
-  is_T_exp (t_of_conf c) && is_E_ffi (e_of_exp (e_of_t_exp (t_of_conf c)))
-
-let pre_ematch (c:config) =
-  is_T_exp (t_of_conf c) && is_E_match (e_of_exp (e_of_t_exp (t_of_conf c)))
-
-(* pre returns comp, for src it's never Skip *)
-type comp = | Do | Skip | NA
-
-val step_aspar_e1: c:config{pre_easpar c} -> Tot config
-let step_aspar_e1 (Conf l m s en (T_exp (Exp (E_aspar e1 e2) _)) tr) =
-  Conf l m ((Frame m en (F_aspar_ps e2) tr)::s) en (T_exp e1) (hide [])
-  
-val step_box_e1: c:config{pre_ebox c} -> Tot config
-let step_box_e1 (Conf l m s en (T_exp (Exp (E_box e1 e2) _)) tr) =
-  Conf l m ((Frame m en (F_box_ps e2) tr)::s) en (T_exp e1) (hide [])
-
-val step_unbox_e: c:config{pre_eunbox c} -> Tot config
-let step_unbox_e (Conf l m s en (T_exp (Exp (E_unbox e) _)) tr) =
-  Conf l m ((Frame m en F_unbox tr)::s) en (T_exp e) (hide [])
- 
-val step_mkwire_e1: c:config{pre_emkwire c} -> Tot config
-let step_mkwire_e1 (Conf l m s en (T_exp (Exp (E_mkwire e1 e2) _)) tr) =
-  Conf l m ((Frame m en (F_mkwire_ps e2) tr)::s) en (T_exp e1) (hide [])
-
-val step_projwire_e1: c:config{pre_eprojwire c} -> Tot config
-let step_projwire_e1 (Conf l m s en (T_exp (Exp (E_projwire e1 e2) _)) tr) =
-  Conf l m ((Frame m en (F_projwire_p e2) tr)::s) en (T_exp e1) (hide [])
-
-val step_concatwire_e1: c:config{pre_econcatwire c} -> Tot config
-let step_concatwire_e1 (Conf l m s en (T_exp (Exp (E_concatwire e1 e2) _)) tr) =
-  Conf l m ((Frame m en (F_concatwire_e1 e2) tr)::s) en (T_exp e1) (hide [])
-
-val step_const: c:config{pre_econst c} -> Tot config
-let step_const (Conf l m s en (T_exp (Exp (E_const c) _)) tr) =
-  Conf l m s en (T_val (V_const c)) tr
-
-val step_var: c:config{pre_evar c} -> Tot config
-let step_var (Conf l m s en (T_exp (Exp (E_var x) _)) tr) =
-  let Some (D_v _ v) = en x in
-  Conf l m s en (T_val v) tr
-
-val step_let_e1: c:config{pre_elet c} -> Tot config
-let step_let_e1 (Conf l m s en (T_exp (Exp (E_let x e1 e2) _)) tr) =
-  Conf l m ((Frame m en (F_let x e2) tr)::s) en (T_exp e1) (hide [])
-
-val step_abs: c:config{pre_eabs c} -> Tot config
-let step_abs (Conf l m s en (T_exp (Exp (E_abs x e) _)) tr) =
-  Conf l m s en (T_val (V_clos en x e)) tr
- 
-val step_fix: c:config{pre_efix c} -> Tot config
-let step_fix (Conf l m s en (T_exp (Exp (E_fix f x e) _)) tr) =
-  Conf l m s en (T_val (V_fix_clos en f x e)) tr
-
-val step_empabs: c:config{pre_eempabs c} -> Tot config
-let step_empabs (Conf l m s en (T_exp (Exp (E_empabs x e) _)) tr) =
-  Conf l m s en (T_val (V_emp_clos x e)) tr
-
-val step_app_e1: c:config{pre_eapp c} -> Tot config
-let step_app_e1 (Conf l m s en (T_exp (Exp (E_app e1 e2) _)) tr) =
-  Conf l m ((Frame m en (F_app_e1 e2) tr)::s) en (T_exp e1) (hide [])
- 
-val step_ffi_e: c:config{pre_effi c} -> Tot config
-let step_ffi_e (Conf l m s en (T_exp (Exp (E_ffi fn es) _)) tr) = match es with
-  | []    -> Conf l m s en (T_red (R_ffi fn [])) tr
-  | e::tl  -> Conf l m ((Frame m en (F_ffi fn tl []) tr)::s) en (T_exp e) (hide [])
-  
-val step_match_e: c:config{pre_ematch c} -> Tot config
-let step_match_e (Conf l m s en (T_exp (Exp (E_match e pats) _)) tr) =
-  Conf l m ((Frame m en (F_match pats) tr)::s) en (T_exp e) (hide [])
-
 val concat_traces: erased trace -> erased trace -> Tot (erased trace)
 let concat_traces t1 t2 = elift2 append t1 t2
-
-(* val append_flat_lemma: t1:trace -> t2:trace *)
-(*                        -> Lemma (requires (is_flat_trace t1 /\ is_flat_trace t2)) *)
-(* 		               (ensures (is_flat_trace (append t1 t2))) *)
-(* 		         [SMTPat (is_flat_trace (append t1 t2))] *)
-(* let rec append_flat_lemma t1 t2 = match t1 with *)
-(*   | []   -> () *)
-(*   | _::tl -> append_flat_lemma tl t2 *)
-
-val step_aspar_e2: c:config{is_value_ps c /\ is_sframe c is_F_aspar_ps}
-                  -> Tot config
-let step_aspar_e2 (Conf l _ ((Frame m en (F_aspar_ps e) tr)::s) _
-                       (T_val (V_const (C_prins ps))) tr') =
-  Conf l m ((Frame m en (F_aspar_e ps) (concat_traces tr tr'))::s) en (T_exp e) (hide [])
 
 val vals_traces_h_append_lemma:
   tr1:trace{vals_trace_h tr1} -> tr2:trace{vals_trace_h tr2}
@@ -186,89 +50,25 @@ let vals_traces_concat_lemma tr1 tr2 =
   let _ = assert (vals_trace_h (append (reveal tr1) (reveal tr2))) in
   ()
 
-val step_box_e2: c:config{is_value_ps c /\ is_sframe c is_F_box_ps}
+//----- aspar e1 e2 -----//
+
+let pre_easpar (c:config) =
+  is_T_exp (t_of_conf c) && is_E_aspar (e_of_exp (e_of_t_exp (t_of_conf c))) && is_par c
+
+val step_aspar_e1: c:config{pre_easpar c} -> Tot config
+let step_aspar_e1 (Conf l m s en (T_exp (Exp (E_aspar e1 e2) _)) tr) =
+  Conf l m ((Frame m en (F_aspar_ps e2) tr)::s) en (T_exp e1) (hide [])
+
+val step_aspar_e2: c:config{is_value_ps c /\ is_sframe c is_F_aspar_ps}
                   -> Tot config
-let step_box_e2 (Conf l _ ((Frame m en (F_box_ps e) tr)::s) _
-                      (T_val (V_const (C_prins ps))) tr') =
-  Conf l m ((Frame m en (F_box_e ps) (concat_traces tr tr'))::s) en (T_exp e) (hide [])
+let step_aspar_e2 (Conf l _ ((Frame m en (F_aspar_ps e) tr)::s) _
+                   (T_val (V_prins ps)) tr') =
+  Conf l m ((Frame m en (F_aspar_e ps) (concat_traces tr tr'))::s) en (T_exp e) (hide [])
 
-val step_mkwire_e2: c:config{is_value c /\ is_sframe c is_F_mkwire_ps}
-                   -> Tot config
-let step_mkwire_e2 (Conf l _ ((Frame m en (F_mkwire_ps e) tr)::s) _
-                        (T_val v) tr') =
-  Conf l m ((Frame m en (F_mkwire_e v) (concat_traces tr tr'))::s) en (T_exp e) (hide [])
-
-val step_projwire_e2: c:config{is_value_p c /\ is_sframe c is_F_projwire_p}
-                     -> Tot config
-let step_projwire_e2 (Conf l _ ((Frame m en (F_projwire_p e) tr)::s) _
-                          (T_val (V_const (C_prin p))) tr') =
-  Conf l m ((Frame m en (F_projwire_e p) (concat_traces tr tr'))::s) en (T_exp e) (hide [])
-
-val step_concatwire_e2: c:config{is_value c /\ is_sframe c is_F_concatwire_e1}
-                       -> Tot config
-let step_concatwire_e2 (Conf l _ ((Frame m en (F_concatwire_e1 e) tr)::s) _
-                            (T_val v) tr') =
-  Conf l m ((Frame m en (F_concatwire_e2 v) (concat_traces tr tr'))::s) en (T_exp e) (hide [])
-
-val step_app_e2: c:config{is_value c /\ is_sframe c is_F_app_e1}
-                -> Tot config
-let step_app_e2 (Conf l _ ((Frame m en (F_app_e1 e2) tr)::s) _ (T_val v) tr') =
-  Conf l m ((Frame m en (F_app_e2 v) (concat_traces tr tr'))::s) en (T_exp e2) (hide [])
-
-val step_ffi_l: c:config{is_value c /\ is_sframe c is_F_ffi} -> Tot config
-let step_ffi_l (Conf l _ ((Frame m en (F_ffi fn es vs) tr)::s) _ (T_val #meta v) tr') =
-  match es with
-    | []    -> Conf l m s en (T_red (R_ffi fn ((D_v meta v)::vs))) (concat_traces tr tr')
-    | e::tl -> Conf l m ((Frame m en (F_ffi fn tl ((D_v meta v)::vs)) (concat_traces tr tr'))::s) en (T_exp e) (hide [])
-    
-val step_match_red: c:config{is_value c /\ is_sframe c is_F_match} -> Tot config
-let step_match_red (Conf l _ ((Frame m en (F_match pats) tr)::s) _ (T_val v) tr') =
-  Conf l m s en (T_red (R_match v pats)) (concat_traces tr tr')
-  
 val step_aspar_red: c:config{is_value c /\ is_sframe c is_F_aspar_e}
                    -> Tot config
 let step_aspar_red (Conf l _ ((Frame m en (F_aspar_e ps) tr)::s) _ (T_val v) tr') =
   Conf l m s en (T_red (R_aspar ps v)) (concat_traces tr tr')
-
-val step_box_red: c:config{is_value c /\ is_sframe c is_F_box_e}
-                   -> Tot config
-let step_box_red (Conf l _ ((Frame m en (F_box_e ps) tr)::s) _ (T_val v) tr') =
-  Conf l m s en (T_red (R_box ps v)) (concat_traces tr tr')
-
-(*val step_box_red: c:config{is_value c /\ is_sframe c is_F_box_e}
-                 -> Tot config
-let step_box_red (Conf l _ ((Frame m en (F_box_e ps))::s) _ (T_val v)) =
-  Conf l m s en (T_red (R_box ps v))*)
-
-val step_unbox_red: c:config{is_value c /\ is_sframe c is_F_unbox}
-                   -> Tot config
-let step_unbox_red (Conf l _ ((Frame m en F_unbox tr)::s) _ (T_val v) tr') =
-  Conf l m s en (T_red (R_unbox v)) (concat_traces tr tr')
-
-val step_projwire_red: c:config{is_value c /\ is_sframe c is_F_projwire_e}
-                      -> Tot config
-let step_projwire_red (Conf l _ ((Frame m en (F_projwire_e p) tr)::s) _ (T_val v) tr') =
-  Conf l m s en (T_red (R_projwire p v)) (concat_traces tr tr')
-
-val step_mkwire_red: c:config{is_value c /\ is_sframe c is_F_mkwire_e}
-                    -> Tot config
-let step_mkwire_red (Conf l _ ((Frame m en (F_mkwire_e v1) tr)::s) _ (T_val v2) tr') =
-  Conf l m s en (T_red (R_mkwire v1 v2)) (concat_traces tr tr')
-
-val step_concatwire_red: c:config{is_value c /\ is_sframe c is_F_concatwire_e2}
-                        -> Tot config
-let step_concatwire_red (Conf l _ ((Frame m en (F_concatwire_e2 v1) tr)::s) _ (T_val v2) tr') =
-  Conf l m s en (T_red (R_concatwire v1 v2)) (concat_traces tr tr')
-
-val step_let_red: c:config{is_value c /\ is_sframe c is_F_let}
-                 -> Tot config
-let step_let_red (Conf l _ ((Frame m en (F_let x e2) tr)::s) _ (T_val v) tr') =
-  Conf l m s en (T_red (R_let x v e2)) (concat_traces tr tr')
-
-val step_app_red: c:config{is_value c /\ is_sframe c is_F_app_e2}
-                 -> Tot config
-let step_app_red (Conf l _ ((Frame m en (F_app_e2 v1) tr)::s) _ (T_val v2) tr') =
-  Conf l m s en (T_red (R_app v1 v2)) (concat_traces tr tr')
 
 val pre_aspar: config -> Tot comp
 let pre_aspar c = match c with
@@ -295,13 +95,60 @@ let step_aspar c = match c with
      * implementation can make whatever decision (retain env as in F* semantics)
      *)
     let en', t' =
-      if src l then update_env en x (V_const C_unit), T_exp e
+      if src l then update_env en x V_unit, T_exp e
       else
-        if pre_aspar c = Do then update_env en x (V_const C_unit), T_exp e
+        if pre_aspar c = Do then update_env en x V_unit, T_exp e
         else empty_env, T_val V_emp
     in
 
     Conf l m' s' en' t' (hide [])
+
+val pre_aspar_ret: config -> Tot comp
+let pre_aspar_ret c = match c with
+  | Conf _ _ ((Frame _ _ (F_aspar_ret ps) _)::_) _ (T_val #meta _) _ ->
+    if is_meta_boxable ps meta then Do else NA
+      (*if src l then
+        if subset ps2 ps1 then Do else NA
+      else Do
+    else NA
+*)
+  | _ -> NA
+
+val scope_trace: prins -> trace -> Tot trace
+let scope_trace ps t = [ Tr_scope ps t ]
+
+val step_aspar_ret: c:config{pre_aspar_ret c = Do} -> Tot config
+let step_aspar_ret c = match c with
+  | Conf l _ ((Frame m en (F_aspar_ret ps) tr)::s) _ (T_val v) tr' ->
+    let tr =
+      if l = Source then
+	concat_traces tr (elift1 (scope_trace ps) tr')
+      else concat_traces tr tr'
+    in
+	
+    Conf l m s en (T_val (V_box ps v)) tr
+
+//----- aspar e1 e2 -----//
+
+// ----- box e1 e2 -----//
+
+let pre_ebox (c:config) =
+  is_T_exp (t_of_conf c) && is_E_box (e_of_exp (e_of_t_exp (t_of_conf c)))
+
+val step_box_e1: c:config{pre_ebox c} -> Tot config
+let step_box_e1 (Conf l m s en (T_exp (Exp (E_box e1 e2) _)) tr) =
+  Conf l m ((Frame m en (F_box_ps e2) tr)::s) en (T_exp e1) (hide [])
+
+val step_box_e2: c:config{is_value_ps c /\ is_sframe c is_F_box_ps}
+                  -> Tot config
+let step_box_e2 (Conf l _ ((Frame m en (F_box_ps e) tr)::s) _
+                 (T_val (V_prins ps)) tr') =
+  Conf l m ((Frame m en (F_box_e ps) (concat_traces tr tr'))::s) en (T_exp e) (hide [])
+
+val step_box_red: c:config{is_value c /\ is_sframe c is_F_box_e}
+                   -> Tot config
+let step_box_red (Conf l _ ((Frame m en (F_box_e ps) tr)::s) _ (T_val v) tr') =
+  Conf l m s en (T_red (R_box ps v)) (concat_traces tr tr')
 
 val pre_box: c:config -> Tot comp
 let pre_box c = match c with
@@ -323,6 +170,173 @@ let step_box (Conf l m s en (T_red (R_box ps' v)) tr) =
     if subset ps ps' then Conf l m s en (T_val (V_box ps' v)) tr
     else Conf l m s en (T_val (V_box ps' V_emp)) tr // TODO: FIXME: V_emp or v ?
 
+//----- box e1 e2 -----//
+
+//----- app e1 e2 -----//
+
+let pre_eapp (c:config) =
+  is_T_exp (t_of_conf c) && is_E_app (e_of_exp (e_of_t_exp (t_of_conf c)))
+
+val step_app_e1: c:config{pre_eapp c} -> Tot config
+let step_app_e1 (Conf l m s en (T_exp (Exp (E_app e1 e2) _)) tr) =
+  Conf l m ((Frame m en (F_app_e1 e2) tr)::s) en (T_exp e1) (hide [])
+
+val step_app_e2: c:config{is_value c /\ is_sframe c is_F_app_e1}
+                -> Tot config
+let step_app_e2 (Conf l _ ((Frame m en (F_app_e1 e2) tr)::s) _ (T_val v) tr') =
+  Conf l m ((Frame m en (F_app_e2 v) (concat_traces tr tr'))::s) en (T_exp e2) (hide [])
+
+val step_app_red: c:config{is_value c /\ is_sframe c is_F_app_e2}
+                 -> Tot config
+let step_app_red (Conf l _ ((Frame m en (F_app_e2 v1) tr)::s) _ (T_val v2) tr') =
+  Conf l m s en (T_red (R_app v1 v2)) (concat_traces tr tr')
+
+val pre_app: c:config -> Tot bool
+let pre_app c = match c with
+  | Conf _ _ _ _ (T_red (R_app v _)) _ -> is_clos v
+
+  | _ -> false
+
+val step_app: c:config{pre_app c} -> Tot config
+let step_app c = match c with
+  | Conf l m s _ (T_red (R_app f v)) tr ->
+    let (en, x, e) = get_en_b f in
+    Conf l m s (update_env en x v) (T_exp e) tr
+
+//----- app e1 e2 -----//
+
+//----- fun x.e -----//
+
+let pre_eabs (c:config) =
+  is_T_exp (t_of_conf c) && is_E_abs (e_of_exp (e_of_t_exp (t_of_conf c)))
+
+val step_abs: c:config{pre_eabs c} -> Tot config
+let step_abs (Conf l m s en (T_exp (Exp (E_abs x e) _)) tr) =
+  Conf l m s en (T_val (V_clos en x e)) tr
+
+//----- fun x.e -----//
+
+//----- fix f.fun x.e -----//
+
+let pre_efix (c:config) =
+  is_T_exp (t_of_conf c) && is_E_fix (e_of_exp (e_of_t_exp (t_of_conf c)))
+
+val step_fix: c:config{pre_efix c} -> Tot config
+let step_fix (Conf l m s en (T_exp (Exp (E_fix f x e) _)) tr) =
+  Conf l m s en (T_val (V_fix_clos en f x e)) tr
+
+//----- fix f.fun x. e -----//
+
+//----- fun x.e (closed) -----//
+
+let pre_eempabs (c:config) =
+  is_T_exp (t_of_conf c) && is_E_empabs (e_of_exp (e_of_t_exp (t_of_conf c)))
+
+val step_empabs: c:config{pre_eempabs c} -> Tot config
+let step_empabs (Conf l m s en (T_exp (Exp (E_empabs x e) _)) tr) =
+  Conf l m s en (T_val (V_emp_clos x e)) tr
+
+//----- fun x.e (closed) -----// 
+
+//----- let x = e1 in e2 -----//
+
+let pre_elet (c:config) =
+  is_T_exp (t_of_conf c) && is_E_let (e_of_exp (e_of_t_exp (t_of_conf c)))
+
+val step_let_e1: c:config{pre_elet c} -> Tot config
+let step_let_e1 (Conf l m s en (T_exp (Exp (E_let x e1 e2) _)) tr) =
+  Conf l m ((Frame m en (F_let x e2) tr)::s) en (T_exp e1) (hide [])
+
+val step_let_red: c:config{is_value c /\ is_sframe c is_F_let}
+                 -> Tot config
+let step_let_red (Conf l _ ((Frame m en (F_let x e2) tr)::s) _ (T_val v) tr') =
+  Conf l m s en (T_red (R_let x v e2)) (concat_traces tr tr')
+
+val pre_let: c:config -> Tot bool
+let pre_let c = match c with
+  | Conf _ _ _ _ (T_red (R_let _ _ _)) _ -> true
+  | _                                    -> false
+
+val step_let: c:config{pre_let c} -> Tot config
+let step_let c = match c with
+  | Conf l m s en (T_red (R_let x v1 e2)) tr ->
+    Conf l m s (update_env en x v1) (T_exp e2) tr
+
+//----- let x = e1 in e2 -----//
+
+//----- x -----//
+
+(* TODO: FIXME: workaround for projectors *)
+val x_of_e_var: e:exp'{is_E_var e} -> Tot varname
+let x_of_e_var (E_var x) = x
+
+(* TODO: FIXME: workaround for projectors *)
+val is_Some: option 'a -> Tot bool
+let is_Some x = match x with
+  | Some _ -> true
+  | _      -> false
+
+(* TODO: FIXME: workaround for projectors *)
+val en_of_conf: config -> Tot env
+let en_of_conf (Conf _ _ _ en _ _) = en
+
+let pre_evar (c:config) =
+  is_T_exp (t_of_conf c) && is_E_var (e_of_exp (e_of_t_exp (t_of_conf c))) &&
+  is_Some ((en_of_conf c) (x_of_e_var (e_of_exp (e_of_t_exp (t_of_conf c)))))
+
+val step_var: c:config{pre_evar c} -> Tot config
+let step_var (Conf l m s en (T_exp (Exp (E_var x) _)) tr) =
+  let Some (D_v _ v) = en x in
+  Conf l m s en (T_val v) tr
+
+//----- x -----//
+
+//----- c -----//
+
+let pre_econst (c:config) =
+  is_T_exp (t_of_conf c) && is_E_const (e_of_exp (e_of_t_exp (t_of_conf c)))
+
+val slice_const: p:prin -> 'a -> Tot 'a
+let slice_const p x = x
+
+val compose_const: 'a -> 'a -> Tot 'a
+let compose_const x _ = x
+
+val slice_const_sps: ps:prins -> 'a -> Tot 'a
+let slice_const_sps ps x = x
+
+val step_const: c:config{pre_econst c} -> Tot config
+let step_const (Conf l m s en (T_exp (Exp (E_const c) _)) tr) =
+  let meta = Meta empty Can_b empty Can_w in
+  let v = match c with
+    | C_prin p     -> V_prin p
+    | C_eprins eps -> V_eprins eps
+    | C_prins ps   -> V_prins ps
+
+    | C_unit _     -> V_unit
+    | C_bool b     -> V_bool b
+
+    | C_opaque 'a v -> V_opaque v meta slice_const compose_const slice_const_sps
+  in
+
+  Conf l m s en (T_val v) tr
+
+//----- c -----//
+
+//----- unbox e -----//
+
+let pre_eunbox (c:config) =
+  is_T_exp (t_of_conf c) && is_E_unbox (e_of_exp (e_of_t_exp (t_of_conf c)))
+
+val step_unbox_e: c:config{pre_eunbox c} -> Tot config
+let step_unbox_e (Conf l m s en (T_exp (Exp (E_unbox e) _)) tr) =
+  Conf l m ((Frame m en F_unbox tr)::s) en (T_exp e) (hide [])
+
+val step_unbox_red: c:config{is_value c /\ is_sframe c is_F_unbox}
+                   -> Tot config
+let step_unbox_red (Conf l _ ((Frame m en F_unbox tr)::s) _ (T_val v) tr') =
+  Conf l m s en (T_red (R_unbox v)) (concat_traces tr tr')
+
 val pre_unbox: config -> Tot comp
 let pre_unbox c = match c with
   | Conf _ (Mode as_m ps1) _ _ (T_red (R_unbox (V_box ps2 _))) _ ->
@@ -337,17 +351,39 @@ val step_unbox: c:config{pre_unbox c = Do} -> Tot config
 let step_unbox c = match c with
   | Conf l m s en (T_red (R_unbox (V_box _ v))) tr -> Conf l m s en (T_val v) tr
 
+//----- unbox e -----//
+
+//----- mkwire e1 e2 -----//
+
+let pre_emkwire (c:config) =
+  is_T_exp (t_of_conf c) && is_E_mkwire (e_of_exp (e_of_t_exp (t_of_conf c)))
+
+val step_mkwire_e1: c:config{pre_emkwire c} -> Tot config
+let step_mkwire_e1 (Conf l m s en (T_exp (Exp (E_mkwire e1 e2) _)) tr) =
+  Conf l m ((Frame m en (F_mkwire_ps e2) tr)::s) en (T_exp e1) (hide [])
+
+val step_mkwire_e2: c:config{is_value c /\ is_sframe c is_F_mkwire_ps}
+                   -> Tot config
+let step_mkwire_e2 (Conf l _ ((Frame m en (F_mkwire_ps e) tr)::s) _
+                    (T_val v) tr') =
+  Conf l m ((Frame m en (F_mkwire_e v) (concat_traces tr tr'))::s) en (T_exp e) (hide [])
+
+val step_mkwire_red: c:config{is_value c /\ is_sframe c is_F_mkwire_e}
+                    -> Tot config
+let step_mkwire_red (Conf l _ ((Frame m en (F_mkwire_e v1) tr)::s) _ (T_val v2) tr') =
+  Conf l m s en (T_red (R_mkwire v1 v2)) (concat_traces tr tr')
+
 val pre_mkwire: config -> Tot comp
 let pre_mkwire c = match c with
-  | Conf l (Mode Par ps) _ _ (T_red (R_mkwire (V_const (C_prins ps'))
-                                                       (V_box #mv ps'' _))) _ ->
+  | Conf l (Mode Par ps) _ _ (T_red (R_mkwire (V_prins ps')
+                                              (V_box #mv ps'' _))) _ ->
     if is_meta_wireable mv then
       if src l then
         if subset ps' ps && subset ps' ps'' then Do else NA
       else Do
     else NA
  
-  | Conf l (Mode Sec ps) _ _ (T_red (R_mkwire #mps #mv (V_const (C_prins ps')) _)) _ ->
+  | Conf l (Mode Sec ps) _ _ (T_red (R_mkwire #mps #mv (V_prins ps') _)) _ ->
     if is_meta_wireable mv then
       if subset ps' ps then Do else NA
     else NA
@@ -361,8 +397,8 @@ let mconst_on eps v = const_on eps v
 
 val step_mkwire: c:config{pre_mkwire c = Do} -> Tot config
 let step_mkwire c = match c with
-  | Conf l (Mode Par ps) s en (T_red (R_mkwire (V_const (C_prins ps'))
-                                                       (V_box _ v))) tr ->
+  | Conf l (Mode Par ps) s en (T_red (R_mkwire (V_prins ps')
+                                               (V_box _ v))) tr ->
     let eps, w =
       if src l then ps', mconst_on ps' v
       else
@@ -372,8 +408,30 @@ let step_mkwire c = match c with
     in
     Conf l (Mode Par ps) s en (T_val (V_wire eps w)) tr
 
-  | Conf l (Mode Sec ps) s en (T_red (R_mkwire (V_const (C_prins ps')) v)) tr ->
+  | Conf l (Mode Sec ps) s en (T_red (R_mkwire (V_prins ps') v)) tr ->
     Conf l (Mode Sec ps) s en (T_val (V_wire ps' (mconst_on ps' v))) tr
+
+//----- mkwire e1 e2 -----//
+
+//----- projwire e1 e2 -----//
+
+let pre_eprojwire (c:config) =
+  is_T_exp (t_of_conf c) && is_E_projwire (e_of_exp (e_of_t_exp (t_of_conf c)))
+
+val step_projwire_e1: c:config{pre_eprojwire c} -> Tot config
+let step_projwire_e1 (Conf l m s en (T_exp (Exp (E_projwire e1 e2) _)) tr) =
+  Conf l m ((Frame m en (F_projwire_p e2) tr)::s) en (T_exp e1) (hide [])
+
+val step_projwire_e2: c:config{is_value_p c /\ is_sframe c is_F_projwire_p}
+                     -> Tot config
+let step_projwire_e2 (Conf l _ ((Frame m en (F_projwire_p e) tr)::s) _
+                      (T_val (V_prin p)) tr') =
+  Conf l m ((Frame m en (F_projwire_e p) (concat_traces tr tr'))::s) en (T_exp e) (hide [])
+
+val step_projwire_red: c:config{is_value c /\ is_sframe c is_F_projwire_e}
+                      -> Tot config
+let step_projwire_red (Conf l _ ((Frame m en (F_projwire_e p) tr)::s) _ (T_val v) tr') =
+  Conf l m s en (T_red (R_projwire p v)) (concat_traces tr tr')
 
 val pre_projwire: config -> Tot comp
 let pre_projwire c = match c with
@@ -393,6 +451,28 @@ val step_projwire: c:config{pre_projwire c = Do} -> Tot config
 let step_projwire c = match c with
   | Conf l m s en (T_red (R_projwire p (V_wire _ w))) tr ->
     Conf l m s en (T_val (v_of_some (select p w))) tr
+
+//----- projwire e1 e2 -----//
+
+//----- concatwire e1 e2 -----//
+
+let pre_econcatwire (c:config) =
+  is_T_exp (t_of_conf c) && is_E_concatwire (e_of_exp (e_of_t_exp (t_of_conf c)))
+
+val step_concatwire_e1: c:config{pre_econcatwire c} -> Tot config
+let step_concatwire_e1 (Conf l m s en (T_exp (Exp (E_concatwire e1 e2) _)) tr) =
+  Conf l m ((Frame m en (F_concatwire_e1 e2) tr)::s) en (T_exp e1) (hide [])
+
+val step_concatwire_e2: c:config{is_value c /\ is_sframe c is_F_concatwire_e1}
+                       -> Tot config
+let step_concatwire_e2 (Conf l _ ((Frame m en (F_concatwire_e1 e) tr)::s) _
+                        (T_val v) tr') =
+  Conf l m ((Frame m en (F_concatwire_e2 v) (concat_traces tr tr'))::s) en (T_exp e) (hide [])
+
+val step_concatwire_red: c:config{is_value c /\ is_sframe c is_F_concatwire_e2}
+                        -> Tot config
+let step_concatwire_red (Conf l _ ((Frame m en (F_concatwire_e2 v1) tr)::s) _ (T_val v2) tr') =
+  Conf l m s en (T_red (R_concatwire v1 v2)) (concat_traces tr tr')
 
 val pre_concatwire: config -> Tot comp
 let pre_concatwire c = match c with
@@ -440,47 +520,27 @@ let step_concatwire c = match c with
   | Conf l m s en (T_red (R_concatwire (V_wire eps1 w1) (V_wire eps2 w2))) tr ->
     Conf l m s en (T_val (V_wire (union eps1 eps2) (compose_wires #eps1 #eps2 w1 w2 eps1))) tr
 
-val is_let_redex: c:config -> Tot bool
-let is_let_redex c = match c with
-  | Conf _ _ _ _ (T_red (R_let _ _ _)) _ -> true
-  | _                                    -> false
+//----- concatwire e1 e2 -----//
 
-val step_let: c:config{is_let_redex c} -> Tot config
-let step_let c = match c with
-  | Conf l m s en (T_red (R_let x v1 e2)) tr ->
-    Conf l m s (update_env en x v1) (T_exp e2) tr
+//----- ffi f l -----//
 
-val is_app_redex: c:config -> Tot bool
-let is_app_redex c = match c with
-  | Conf _ _ _ _ (T_red (R_app v _)) _ -> is_clos v
+let pre_effi (c:config) =
+  is_T_exp (t_of_conf c) && is_E_ffi (e_of_exp (e_of_t_exp (t_of_conf c)))
 
-  | _ -> false
+val step_ffi_e: c:config{pre_effi c} -> Tot config
+let step_ffi_e (Conf l m s en (T_exp (Exp (E_ffi fn es) _)) tr) = match es with
+  | []    -> Conf l m s en (T_red (R_ffi fn [])) tr
+  | e::tl  -> Conf l m ((Frame m en (F_ffi fn tl []) tr)::s) en (T_exp e) (hide [])
 
-val step_app: c:config{is_app_redex c} -> Tot config
-let step_app c = match c with
-  | Conf l m s _ (T_red (R_app f v)) tr ->
-    let (en, x, e) = get_en_b f in
-    Conf l m s (update_env en x v) (T_exp e) tr
-
-val is_valid_ffi_v: #meta:v_meta -> v:value meta -> Tot bool
-let is_valid_ffi_v #meta v = match v with
-  | V_const _          -> true
-  | V_box _ _          -> false
-  | V_wire _ _         -> false
-  | V_clos _ _ _       -> false
-  | V_fix_clos _ _ _ _ -> false
-  | V_emp_clos _ _     -> false
-  | V_emp              -> false
-
-val is_valid_ffi_vs: list dvalue -> Tot bool
-let rec is_valid_ffi_vs vs = match vs with
-  | []            -> true
-  | (D_v _ v)::tl -> is_valid_ffi_v v && is_valid_ffi_vs tl
+val step_ffi_l: c:config{is_value c /\ is_sframe c is_F_ffi} -> Tot config
+let step_ffi_l (Conf l _ ((Frame m en (F_ffi fn es vs) tr)::s) _ (T_val #meta v) tr') =
+  match es with
+    | []    -> Conf l m s en (T_red (R_ffi fn ((D_v meta v)::vs))) (concat_traces tr tr')
+    | e::tl -> Conf l m ((Frame m en (F_ffi fn tl ((D_v meta v)::vs)) (concat_traces tr tr'))::s) en (T_exp e) (hide [])
 
 val pre_ffi: config -> Tot comp
 let pre_ffi c = match c with
   | Conf _ _ _ _ (T_red (R_ffi _ vs)) _ -> Do
-    (*if is_valid_ffi_vs vs then Do else NA*)
   
   | _ -> NA
 
@@ -489,56 +549,35 @@ let step_ffi (Conf l m s en (T_red (R_ffi fn vs)) tr) =
   let D_v _ v = FFI.exec_ffi fn vs in
   Conf l m s en (T_val v) tr
 
-val pre_match: config -> Tot comp
-let pre_match c = match c with
-  | Conf _ _ _ _ (T_red (R_match _ _)) _ -> Do
+//----- ffi v l -----//
+
+//----- if e then e1 else e2 -----//
+
+let pre_econd (c:config) =
+  is_T_exp (t_of_conf c) && is_E_cond (e_of_exp (e_of_t_exp (t_of_conf c)))
+
+val step_cond_e: c:config{pre_econd c} -> Tot config
+let step_cond_e (Conf l m s en (T_exp (Exp (E_cond e e1 e2) _)) tr) =
+  Conf l m ((Frame m en (F_cond e1 e2) tr)::s) en (T_exp e) (hide [])
+
+val step_cond_red: c:config{is_value c /\ is_sframe c is_F_cond} -> Tot config
+let step_cond_red (Conf l _ ((Frame m en (F_cond e1 e2) tr)::s) _ (T_val v) tr') =
+  Conf l m s en (T_red (R_cond v e1 e2)) (concat_traces tr tr')
+
+val pre_cond: c:config -> Tot bool
+let pre_cond c = match c with
+  | Conf _ _ _ _ (T_red (R_cond (V_bool _) _ _)) _ -> true
+  | _ -> false
+
+val step_cond: c:config{pre_cond c} -> Tot config
+let step_cond c = match c with
+  | Conf l m s en (T_red (R_cond (V_bool b) e1 e2)) tr ->
+    let e = if b then e1 else e2 in
+    Conf l m s en (T_exp e) tr
+
+//----- if e then e1 else e2 -----//
   
-  | _ -> NA
-
-val match_pat: #meta:v_meta -> pat -> value meta -> Tot bool
-let match_pat #meta p v = match p with
-  | P_const pc ->
-    let b =
-    match v with
-      | V_const vc -> pc = vc
-      | _          -> false
-    in
-    b
-
-val get_next_exp: #meta:v_meta -> list (pat * exp) -> value meta -> Tot exp
-let rec get_next_exp #meta pats v = match pats with
-  | []         -> Exp (E_const C_unit) None    // this case should NEVER arise because of exhaustiveness check in F*
-  | (p, e)::tl ->
-    if match_pat p v then e else get_next_exp #meta tl v
-
-val step_match: c:config{pre_match c = Do} -> Tot config
-let step_match (Conf l m s en (T_red (R_match v pats)) tr) =
-  Conf l m s en (T_exp (get_next_exp pats v)) tr
-
-val pre_aspar_ret: config -> Tot comp
-let pre_aspar_ret c = match c with
-  | Conf _ _ ((Frame _ _ (F_aspar_ret ps) _)::_) _ (T_val #meta _) _ ->
-    if is_meta_boxable ps meta then Do else NA
-      (*if src l then
-        if subset ps2 ps1 then Do else NA
-      else Do
-    else NA
-*)
-  | _ -> NA
-
-val scope_trace: prins -> trace -> Tot trace
-let scope_trace ps t = [ Tr_scope ps t ]
-
-val step_aspar_ret: c:config{pre_aspar_ret c = Do} -> Tot config
-let step_aspar_ret c = match c with
-  | Conf l _ ((Frame m en (F_aspar_ret ps) tr)::s) _ (T_val v) tr' ->
-    let tr =
-      if l = Source then
-	concat_traces tr (elift1 (scope_trace ps) tr')
-      else concat_traces tr tr'
-    in
-	
-    Conf l m s en (T_val (V_box ps v)) tr
+//----- assec e1 e2 -----//
 
 let pre_eassec (c:config) =
   is_T_exp (t_of_conf c) && is_E_assec (e_of_exp (e_of_t_exp (t_of_conf c)))
@@ -550,7 +589,7 @@ let step_assec_e1 (Conf l m s en (T_exp (Exp (E_assec e1 e2) _)) tr) =
 val step_assec_e2: c:config{is_value_ps c /\ is_sframe c is_F_assec_ps}
                   -> Tot config
 let step_assec_e2 (Conf l _ ((Frame m en (F_assec_ps e) tr)::s) _
-                       (T_val (V_const (C_prins ps))) tr') =
+                   (T_val (V_prins ps)) tr') =
   Conf l m ((Frame m en (F_assec_e ps) (concat_traces tr tr'))::s) en (T_exp e) (hide [])
 
 val step_assec_red: c:config{is_value c /\ is_sframe c is_F_assec_e}
@@ -574,7 +613,7 @@ let step_assec c = match c with
   | Conf l m s en' (T_red (R_assec ps v)) tr ->
     let (en, x, e) = get_en_b v in
     Conf l (Mode Sec ps) ((Frame m en' F_assec_ret tr)::s)
-           (update_env en x (V_const C_unit)) (T_exp e) (hide [])
+           (update_env en x V_unit) (T_exp e) (hide [])
 
 val step_assec_ret: c:config{is_value c /\ is_sframe c is_F_assec_ret}
                    -> Tot config
@@ -585,29 +624,113 @@ let step_assec_ret (Conf l _ ((Frame m en F_assec_ret tr)::s) _ t tr') =
   in
   Conf l m s en t tr'
 
+//----- assec e1 e2 -----//
+
 type sstep: config -> config -> Type =
   | C_aspar_ps:
     c:config{pre_easpar c} -> c':config{c' = step_aspar_e1 c}
+    -> sstep c c'
+
+  | C_aspar_e:
+    c:config{is_value_ps c /\ is_sframe c is_F_aspar_ps}
+    -> c':config{c' = step_aspar_e2 c}
+    -> sstep c c'
+    
+  | C_aspar_red:
+    c:config{is_value c /\ is_sframe c is_F_aspar_e}
+    -> c':config{c' = step_aspar_red c}
+    -> sstep c c'
+
+  | C_aspar_beta:
+    c:config{not (pre_aspar c = NA)} -> c':config{c' = step_aspar c}
+    -> sstep c c'
+
+  | C_aspar_ret:
+    c:config{is_sframe c is_F_aspar_ret /\ pre_aspar_ret c = Do}
+    -> c':config{c' = step_aspar_ret c}
     -> sstep c c'
     
   | C_box_ps:
     c:config{pre_ebox c} -> c':config{c' = step_box_e1 c}
     -> sstep c c'
 
-  | C_unbox:
-    c:config{pre_eunbox c} -> c':config{c' = step_unbox_e c}
+  | C_box_e:
+    c:config{is_value_ps c /\ is_sframe c is_F_box_ps}
+    -> c':config{c' = step_box_e2 c}
     -> sstep c c'
-   
+
+  | C_box_red:
+    c:config{is_value c /\ is_sframe c is_F_box_e}
+    -> c':config{c' = step_box_red c}
+    -> sstep c c'
+
+  | C_box_beta:
+    c:config{pre_box c = Do} -> c':config{c' = step_box c} -> sstep c c'
+
+  | C_unbox:
+    c:config{pre_eunbox c} -> c':config{c' = step_unbox_e c} -> sstep c c'
+
+  | C_unbox_red:
+    c:config{is_value c /\ is_sframe c is_F_unbox}
+    -> c':config{c' = step_unbox_red c}
+    -> sstep c c'
+
+  | C_unbox_beta:
+    c:config{pre_unbox c = Do} -> c':config{c' = step_unbox c}
+    -> sstep c c'
+
   | C_mkwire_e1:
     c:config{pre_emkwire c} -> c':config{c' = step_mkwire_e1 c}
+    -> sstep c c'
+
+  | C_mkwire_e2:
+    c:config{is_value c /\ is_sframe c is_F_mkwire_ps}
+    -> c':config{c' = step_mkwire_e2 c}
+    -> sstep c c'
+
+  | C_mkwire_red:
+    c:config{is_value c /\ is_sframe c is_F_mkwire_e}
+    -> c':config{c' = step_mkwire_red c}
+    -> sstep c c'
+
+  | C_mkwire_beta:
+    c:config{pre_mkwire c = Do} -> c':config{c' = step_mkwire c}
     -> sstep c c'
 
   | C_projwire_p:
     c:config{pre_eprojwire c} -> c':config{c' = step_projwire_e1 c}
     -> sstep c c'
+
+  | C_projwire_e:
+    c:config{is_value_p c /\ is_sframe c is_F_projwire_p}
+    -> c':config{c' = step_projwire_e2 c}
+    -> sstep c c'
+
+  | C_projwire_red:
+    c:config{is_value c /\ is_sframe c is_F_projwire_e}
+    -> c':config{c' = step_projwire_red c}
+    -> sstep c c'
+
+  | C_projwire_beta:
+    c:config{pre_projwire c = Do} -> c':config{c' = step_projwire c}
+    -> sstep c c'
    
   | C_concatwire_e1:
     c:config{pre_econcatwire c} -> c':config{c' = step_concatwire_e1 c}
+    -> sstep c c'
+
+  | C_concatwire_e2:
+    c:config{is_value c /\ is_sframe c is_F_concatwire_e1}
+    -> c':config{c' = step_concatwire_e2 c}
+    -> sstep c c'
+
+  | C_concatwire_red:
+    c:config{is_value c /\ is_sframe c is_F_concatwire_e2}
+    -> c':config{c' = step_concatwire_red c}
+    -> sstep c c'
+
+  | C_concatwire_beta:
+    c:config{pre_concatwire c = Do} -> c':config{c' = step_concatwire c}
     -> sstep c c'
 
   | C_const:
@@ -621,6 +744,14 @@ type sstep: config -> config -> Type =
   | C_let_e1:
     c:config{pre_elet c} -> c':config{c' = step_let_e1 c}
     -> sstep c c'
+
+  | C_let_red:
+    c:config{is_value c /\ is_sframe c is_F_let}
+    -> c':config{c' = step_let_red c}
+    -> sstep c c'
+
+  | C_let_beta:
+    c:config{pre_let c} -> c':config{c' = step_let c} -> sstep c c'
 
   | C_abs:
     c:config{pre_eabs c} -> c':config{c' = step_abs c}
@@ -637,84 +768,10 @@ type sstep: config -> config -> Type =
   | C_app_e1:
     c:config{pre_eapp c} -> c':config{c' = step_app_e1 c}
     -> sstep c c'
-   
-  | C_ffi_e:
-    c:config{pre_effi c} -> c':config{c' = step_ffi_e c} -> sstep c c'
-    
-  | C_match_e:
-    c:config{pre_ematch c} -> c':config{c' = step_match_e c} -> sstep c c'
-
-  | C_aspar_e:
-    c:config{is_value_ps c /\ is_sframe c is_F_aspar_ps}
-    -> c':config{c' = step_aspar_e2 c}
-    -> sstep c c'
-    
-  | C_box_e:
-    c:config{is_value_ps c /\ is_sframe c is_F_box_ps}
-    -> c':config{c' = step_box_e2 c}
-    -> sstep c c'
-   
-  | C_mkwire_e2:
-    c:config{is_value c /\ is_sframe c is_F_mkwire_ps}
-    -> c':config{c' = step_mkwire_e2 c}
-    -> sstep c c'
- 
-  | C_projwire_e:
-    c:config{is_value_p c /\ is_sframe c is_F_projwire_p}
-    -> c':config{c' = step_projwire_e2 c}
-    -> sstep c c'
-
-  | C_concatwire_e2:
-    c:config{is_value c /\ is_sframe c is_F_concatwire_e1}
-    -> c':config{c' = step_concatwire_e2 c}
-    -> sstep c c'
 
   | C_app_e2:
     c:config{is_value c /\ is_sframe c is_F_app_e1}
     -> c':config{c' = step_app_e2 c}
-    -> sstep c c'
-   
-  | C_ffi_l:
-    c:config{is_value c /\ is_sframe c is_F_ffi}
-    -> c':config{c' = step_ffi_l c} -> sstep c c'
-    
-  | C_match_red:
-    c:config{is_value c /\ is_sframe c is_F_match}
-    -> c':config{c' = step_match_red c} -> sstep c c'
-
-  | C_aspar_red:
-    c:config{is_value c /\ is_sframe c is_F_aspar_e}
-    -> c':config{c' = step_aspar_red c}
-    -> sstep c c'
-
-  | C_box_red:
-    c:config{is_value c /\ is_sframe c is_F_box_e}
-    -> c':config{c' = step_box_red c}
-    -> sstep c c'
-
-  | C_unbox_red:
-    c:config{is_value c /\ is_sframe c is_F_unbox}
-    -> c':config{c' = step_unbox_red c}
-    -> sstep c c'
-   
-  | C_mkwire_red:
-    c:config{is_value c /\ is_sframe c is_F_mkwire_e}
-    -> c':config{c' = step_mkwire_red c}
-    -> sstep c c'
-   
-  | C_projwire_red:
-    c:config{is_value c /\ is_sframe c is_F_projwire_e}
-    -> c':config{c' = step_projwire_red c}
-    -> sstep c c'
-
-  | C_concatwire_red:
-    c:config{is_value c /\ is_sframe c is_F_concatwire_e2}
-    -> c':config{c' = step_concatwire_red c}
-    -> sstep c c'
-
-  | C_let_red:
-    c:config{is_value c /\ is_sframe c is_F_let}
-    -> c':config{c' = step_let_red c}
     -> sstep c c'
 
   | C_app_red:
@@ -722,45 +779,29 @@ type sstep: config -> config -> Type =
     -> c':config{c' = step_app_red c}
     -> sstep c c'
 
-  | C_let_beta:
-    c:config{is_let_redex c} -> c':config{c' = step_let c} -> sstep c c'
-
   | C_app_beta:
-    c:config{is_app_redex c} -> c':config{c' = step_app c} -> sstep c c'
+    c:config{pre_app c} -> c':config{c' = step_app c} -> sstep c c'
    
+  | C_ffi_e:
+    c:config{pre_effi c} -> c':config{c' = step_ffi_e c} -> sstep c c'
+
+  | C_ffi_l:
+    c:config{is_value c /\ is_sframe c is_F_ffi}
+    -> c':config{c' = step_ffi_l c} -> sstep c c'
+
   | C_ffi_beta:
     c:config{pre_ffi c = Do} -> c':config{c' = step_ffi c} -> sstep c c'
-    
-  | C_match_beta:
-    c:config{pre_match c = Do} -> c':config{c' = step_match c} -> sstep c c'
 
-  | C_aspar_beta:
-    c:config{not (pre_aspar c = NA)} -> c':config{c' = step_aspar c}
+  | C_cond_e:
+    c:config{pre_econd c} -> c':config{c' = step_cond_e c} -> sstep c c'
+
+  | C_cond_red:
+    c:config{is_value c /\ is_sframe c is_F_cond}
+    -> c':config{c' = step_cond_red c}
     -> sstep c c'
 
-  | C_box_beta:
-    c:config{pre_box c = Do} -> c':config{c' = step_box c} -> sstep c c'
-
-  | C_unbox_beta:
-    c:config{pre_unbox c = Do} -> c':config{c' = step_unbox c}
-    -> sstep c c'
-   
-  | C_mkwire_beta:
-    c:config{pre_mkwire c = Do} -> c':config{c' = step_mkwire c}
-    -> sstep c c'
-   
-  | C_projwire_beta:
-    c:config{pre_projwire c = Do} -> c':config{c' = step_projwire c}
-    -> sstep c c'
-   
-  | C_concatwire_beta:
-    c:config{pre_concatwire c = Do} -> c':config{c' = step_concatwire c}
-    -> sstep c c'
-    
-  | C_aspar_ret:
-    c:config{is_sframe c is_F_aspar_ret /\ pre_aspar_ret c = Do}
-    -> c':config{c' = step_aspar_ret c}
-    -> sstep c c'
+  | C_cond_beta:
+    c:config{pre_cond c} -> c':config{c' = step_cond c} -> sstep c c'
    
   | C_assec_ps:
     c:config{pre_eassec c} -> c':config{c' = step_assec_e1 c}
@@ -786,8 +827,9 @@ type sstep: config -> config -> Type =
     -> sstep c c'
 
 type slice_v_meta_inv (meta:v_meta) (smeta:v_meta) =
-  subset (Meta.vps smeta) (Meta.vps meta) && (Meta.cb smeta = Meta.cb meta) &&
-  subset (Meta.wps smeta) (Meta.wps meta) && (Meta.cw smeta = Meta.cw meta)
+  (meta = Meta empty Can_b empty Can_w ==> smeta = meta) /\
+  subset (Meta.bps smeta) (Meta.bps meta) /\ (Meta.cb smeta = Meta.cb meta) /\
+  subset (Meta.wps smeta) (Meta.wps meta) /\ (Meta.cw smeta = Meta.cw meta)
 
 opaque val slice_wire:
   #eps:eprins -> p:prin -> w:v_wire eps
@@ -805,22 +847,34 @@ let rec slice_v #meta p v =
   let def = D_v meta v in
   let emp = D_v (Meta empty Can_b empty Can_w) V_emp in
   match v with
-    | V_const _           -> def
+    | V_prin _                  -> def
+    | V_eprins _                -> def
+    | V_prins _                 -> def
 
-    | V_box ps v          ->
+    | V_unit                    -> def
+    | V_bool _                  -> def
+
+    | V_opaque 'a v' m' s c sps  ->
+      let Meta bps cb wps cw = m' in
+      let v'' = s p v' in
+      let m'' = Meta bps cb (intersect wps (singleton p)) cw in
+      let _ = admitP (wps = empty ==> intersect wps (singleton p) = empty) in
+      D_v m'' (V_opaque v'' m'' s c sps)
+
+    | V_box ps v                ->
       let D_v meta' v' = if mem p ps then slice_v p v else emp in
       D_v (Meta ps Can_b (Meta.wps meta') Cannot_w) (V_box ps v')
 
-    | V_wire eps w        -> D_v (Meta empty Can_b (intersect eps (singleton p)) Cannot_w)
-                                 (V_wire (intersect eps (singleton p)) (slice_wire #eps p w))
+    | V_wire eps w              -> D_v (Meta empty Can_b (intersect eps (singleton p)) Cannot_w)
+                                      (V_wire (intersect eps (singleton p)) (slice_wire #eps p w))
 
-    | V_clos en x e       -> D_v meta (V_clos (slice_en p en) x e)
+    | V_clos en x e             -> D_v meta (V_clos (slice_en p en) x e)
 
-    | V_fix_clos en f x e -> D_v meta (V_fix_clos (slice_en p en) f x e)
+    | V_fix_clos en f x e       -> D_v meta (V_fix_clos (slice_en p en) f x e)
 
-    | V_emp_clos _ _      -> def
+    | V_emp_clos _ _            -> def
 
-    | V_emp               -> emp
+    | V_emp                     -> emp
 
 and slice_en p en =
   let _ = () in
@@ -830,10 +884,20 @@ and slice_en p en =
              Some (slice_v p (D_v.v (Some.v (en x))))
 
 type compose_v_meta_inv (m1:v_meta) (m2:v_meta) (cmeta:v_meta) =
- subset (Meta.vps cmeta) (union (Meta.vps m1) (Meta.vps m2))            /\
- ((Meta.cb m1 = Can_b /\ Meta.cb m2 = Can_b) ==> Meta.cb cmeta = Can_b) /\
+ subset (Meta.bps cmeta) (union (Meta.bps m1) (Meta.bps m2))            /\
+ ((Meta.cb m1 = Can_b /\ Meta.cb m2 = Can_b) ==> Meta.cb cmeta = Can_b)   /\
  subset (Meta.wps cmeta) (union (Meta.wps m1) (Meta.wps m2))            /\
  ((Meta.cw m1 = Can_w /\ Meta.cw m2 = Can_w) ==> Meta.cw cmeta = Can_w)
+
+val compose_opaque_meta: m1:v_meta -> m2:v_meta -> Tot (r:v_meta{compose_v_meta_inv m1 m2 r})
+let compose_opaque_meta m1 m2 =
+  let Meta bps1 cb1 wps1 cw1 = m1 in
+  let Meta bps2 cb2 wps2 cw2 = m2 in
+
+  let cb = if cb1 = Can_b && cb2 = Can_b then Can_b else Cannot_b in
+  let cw = if cw1 = Can_w && cw2 = Can_w then Can_w else Cannot_w in
+
+  Meta (union bps1 bps2) cb (union wps1 wps2) cw
 
 (* TODO: FIXME: discriminators are not generated properly, they don't have index argument *)
 val is_v_emp: #meta:v_meta -> v:value meta -> Tot bool
@@ -841,10 +905,35 @@ let is_v_emp #meta v = match v with
   | V_emp -> true
   | _     -> false
 
-val is_v_const: #meta:v_meta -> v:value meta -> Tot bool
-let is_v_const #meta v = match v with
-  | V_const _ -> true
+val is_v_prin: #meta:v_meta -> v:value meta -> Tot bool
+let is_v_prin #meta v = match v with
+  | V_prin _ -> true
+  | _        -> false
+
+val is_v_eprins: #meta:v_meta -> v:value meta -> Tot bool
+let is_v_eprins #meta v = match v with
+  | V_eprins _ -> true
+  | _          -> false
+
+val is_v_prins: #meta:v_meta -> v:value meta -> Tot bool
+let is_v_prins #meta v = match v with
+  | V_prins _ -> true
   | _         -> false
+
+val is_v_unit: #meta:v_meta -> v:value meta -> Tot bool
+let is_v_unit #meta v = match v with
+  | V_unit   -> true
+  | _        -> false
+
+val is_v_bool: #meta:v_meta -> v:value meta -> Tot bool
+let is_v_bool #meta v = match v with
+  | V_bool _ -> true
+  | _        -> false
+
+val is_v_opaque: #meta:v_meta -> v:value meta -> Tot bool
+let is_v_opaque #meta v = match v with
+  | V_opaque 'a _ _ _ _ _ -> true
+  | _                    -> false
 
 val is_v_box: #meta:v_meta -> v:value meta -> Tot bool
 let is_v_box #meta v = match v with
@@ -871,6 +960,9 @@ let is_v_emp_clos #meta v = match v with
   | V_emp_clos _ _ -> true
   | _              -> false
 
+type compose_fn_wrapper =
+  | Mk_c_w: ('a -> 'a -> Tot 'a) -> compose_fn_wrapper
+
 val compose_vals: #m1:v_meta -> #m2:v_meta -> v1:value m1 -> v2:value m2
                  -> Tot (r:dvalue{compose_v_meta_inv m1 m2 (D_v.meta r)})
                     (decreases %[v1])
@@ -882,9 +974,41 @@ let rec compose_vals #m1 #m2 v1 v2 =
  else
    let emp = D_v (Meta empty Can_b empty Can_w) V_emp in
    match v1 with
-     | V_const c1 ->
-       if is_v_const v2 && V_const.c v1 = V_const.c v2 then
-         D_v m1 v1
+     | V_prin p1 ->
+       if is_v_prin v2 && V_prin.c v1 = V_prin.c v2 then
+	 D_v m1 v1
+       else emp
+       
+     | V_eprins eps1 ->
+       if is_v_eprins v2 && V_eprins.c v1 = V_eprins.c v2 then
+	 D_v m1 v1
+       else emp
+
+     | V_prins ps1 ->
+       if is_v_prins v2 && V_prins.c v1 = V_prins.c v2 then
+	 D_v m1 v1
+       else emp
+
+     | V_unit ->
+       if is_v_unit v2 then
+	 D_v m1 v1
+       else emp
+
+     | V_bool b1 ->
+       if is_v_bool v2 && V_bool.c v1 = V_bool.c v2 then
+	 D_v m1 v1
+       else emp
+
+     | V_opaque 'a v1 m1 s1 c1 sps1 ->
+       if is_v_opaque v2 then
+	 let V_opaque 'b v2 m2 s2 c2 sps2 = v2 in
+	 let c1' = Mk_c_w c1 in
+	 let c2' = Mk_c_w c2 in
+	 if c1' = c2' then
+	   let v' = c1 v1 v2 in
+	   let m' = compose_opaque_meta m1 m2 in
+	   D_v m' (V_opaque v' m' s1 c1 sps1)
+	 else emp
        else emp
 
      | V_box ps1 v1 ->
